src/DefineAbsR.v
@@ -24,44 +24,21 @@ Lemma find_define : forall Word8 addr len pos v w m,
                                     (fun i => M.add (addr + i)%N w) len).
 Proof.
   intros.
-  decisions; subst.
-    apply Bool.andb_true_iff in Heqe.
-    destruct Heqe.
-    undecide.
-    induction len using N.peano_ind; simpl in *.
-      rewrite N.add_0_r in H0.
-      nomega.
-    rewrite N.peano_rect_succ.
+  decisions; subst;
+  induction len using N.peano_ind; simpl in *; trivial.
+  - nomega.
+  - rewrite N.peano_rect_succ.
     destruct (N.eq_dec pos (addr + len)); subst.
       intuition.
     apply F.add_mapsto_iff.
     right; split; trivial.
-      apply not_eq_sym; assumption.
-    rewrite N.add_succ_r in H0.
-    apply N.lt_succ_r in H0.
-    pose proof (proj2 (N.le_neq pos (addr + len)) (conj H0 n)).
-    apply IHlen; assumption.
-  apply Bool.andb_false_iff in Heqe.
-  destruct Heqe; undecide;
-  induction len using N.peano_ind; simpl in *; auto;
-  rewrite N.peano_rect_succ.
+      nomega.
+    apply IHlen; nomega.
+  - rewrite N.peano_rect_succ.
     simplify_maps.
     right; split; trivial.
-    unfold not; intros; subst.
-    rewrite <- (N.add_0_r addr) in H0 at 2.
-    apply N.add_lt_cases in H0.
-    destruct H0.
       nomega.
-    contradiction (N.nlt_0_r len).
-  rewrite N.add_succ_r in H0.
-  simplify_maps.
-  right; split.
-    unfold not; intros; subst.
-    apply N.le_succ_l in H0.
-    nomega.
-  apply IHlen.
-  apply N.le_succ_l in H0.
-  nomega.
+    apply IHlen; nomega.
 Qed.
 
 Lemma Nle_ne_succ : forall n m,
@@ -82,62 +59,9 @@ Lemma find_define_inv : forall Word8 addr len pos v w m,
 Proof.
   intros.
   induction len using N.peano_ind; simpl in *;
-  decisions; auto.
-  - apply Bool.andb_true_iff in Heqe;
-    destruct Heqe; undecide.
-    rewrite N.add_0_r in H1.
-    nomega.
-  - rewrite N.peano_rect_succ in H.
-    simplify_maps; auto.
-  - rewrite N.peano_rect_succ in H.
-    simplify_maps; auto.
-      nomega.
-    apply Bool.andb_true_iff in Heqe;
-    destruct Heqe; undecide.
-    apply Bool.andb_false_iff in Heqe0;
-    destruct Heqe0; undecide.
-      nomega.
-    intuition; subst.
-    rewrite N.add_succ_r in H1.
-    apply N.le_succ_l in H1.
-    nomega.
-  - rewrite N.peano_rect_succ in H.
-    simplify_maps; auto.
-    intuition.
-    apply Bool.andb_true_iff in Heqe0;
-    destruct Heqe0; undecide.
-    apply Bool.andb_false_iff in Heqe;
-    destruct Heqe; undecide.
-      nomega.
-    rewrite N.add_succ_r in H1.
-    apply not_eq_sym in H3.
-    pose proof (Nle_ne_succ H3 H1).
-    nomega.
-  - rewrite N.peano_rect_succ in H.
-    simplify_maps; auto.
-    intuition.
-    apply Bool.andb_false_iff in Heqe0;
-    destruct Heqe0; undecide;
-    apply Bool.andb_false_iff in Heqe;
-    destruct Heqe; undecide.
-    + rewrite <- N.add_0_r in H0.
-      apply N.add_lt_cases in H0.
-      destruct H0.
-        nomega.
-      contradiction (N.nlt_0_r len).
-    + rewrite <- N.add_0_r in H.
-      apply N.add_lt_cases in H.
-      destruct H.
-        nomega.
-      contradiction (N.nlt_0_r len).
-    + rewrite <- N.add_0_r in H0.
-      apply N.add_lt_cases in H0.
-      destruct H0.
-        nomega.
-      contradiction (N.nlt_0_r len).
-    + rewrite N.add_succ_r in H.
-      apply N.le_succ_l in H.
-      nomega.
+  decisions; auto; try nomega;
+  rewrite N.peano_rect_succ in H;
+  simplify_maps; nomega.
 Qed.
 
 Lemma Define_Map_AbsR : forall Word8 x y b len w,
@@ -153,45 +77,37 @@ Proof.
     exists blk; intuition;
     apply find_define;
     unfold IfDec_Then_Else; simpl.
-      apply within_reflect in H0.
-      rewrite H0; reflexivity.
-    apply not_within_reflect in H0.
-    rewrite H0.
-    apply H.
-    exists blk; intuition.
+      decisions; nomega.
+    decisions.
+      contradiction H0; nomega.
+    apply H; firstorder.
   - reduction.
     apply find_define_inv in H0.
     decisions; auto; subst.
-      left.
-      apply within_reflect in Heqe.
-      intuition.
-    right.
-    apply not_within_reflect in Heqe.
+      left; intuition; nomega.
+    right; intuition.
+      nomega.
     apply H in H0.
     destruct H0, H0; subst.
     intuition.
   - reduction.
     apply find_define_inv in H0.
     decisions; auto; subst.
-      apply within_reflect in Heqe.
-      exists w; intuition.
-      teardown.
-      left; intuition.
-    apply not_within_reflect in Heqe.
+      exists w; intuition; teardown.
+      left; intuition; nomega.
     apply H in H0.
     destruct H0, H0; subst.
-    exists cblk; intuition.
-    teardown.
-    right; intuition.
+    exists cblk; intuition; teardown.
+    right; intuition; nomega.
   - repeat teardown; subst; [inv H2|];
     apply find_define;
     unfold IfDec_Then_Else; simpl.
-      apply within_reflect in H0.
-      rewrite H0; reflexivity.
-    apply not_within_reflect in H0.
-    rewrite H0.
-    apply H.
-    exists cblk; intuition.
+      decisions; nomega.
+    apply H in H2.
+    decisions.
+      nomega.
+    destruct H2, H1; subst.
+    intuition.
 Qed.
 
 End Define_AbsR.
