src/Nomega.v
@@ -1,192 +1,111 @@
-Require Import
-  Fiat.ADT
-  Fiat.ADTNotation.
-
 Require Export
+  Coq.Arith.Arith
+  Coq.omega.Omega
   Coq.NArith.NArith
-  Omega.
-
-Require Export
   Here.Decidable.
 
 Open Scope N_scope.
 
-Definition within (addr : N) (len : N) (a : N) : Prop :=
-  addr <= a < addr + len.
+Hint Rewrite
+  Nplus_0_r
+  nat_of_Nsucc
+  nat_of_Nplus
+  nat_of_Nminus
+  N_of_nat_of_N
+  nat_of_N_of_nat
+  nat_of_P_o_P_of_succ_nat_eq_succ
+  nat_of_P_succ_morphism : N.
 
-Definition within_le (addr : N) (len : N) (a : N) : Prop :=
-  addr <= a <= addr + len.
+Corollary sumbool_split : forall P Q : Prop,
+  {P} + {~P} -> {Q} + {~Q} -> {P /\ Q} + {~ (P /\ Q)}.
+Proof. intros; intuition. Qed.
 
-Lemma within_refl : forall addr len,
-  0 < len -> within addr len addr.
+Section N_theory.
+
+Variables n m : N.
+
+Theorem Neq_in : nat_of_N n = nat_of_N m -> n = m.
 Proof.
-  split; intros.
-    apply N.le_refl.
-  apply N.lt_add_pos_r.
-  assumption.
+  intros H; apply (f_equal N_of_nat) in H;
+  autorewrite with N in *; assumption.
 Qed.
 
-Definition fits (addr1 len1 addr2 len2 : N) : Prop :=
-  within addr1 len1 addr2 /\ within addr1 len1 (addr2 + len2).
-
-Definition overlaps (addr len addr2 len2 : N) : Prop :=
-  addr < addr2 + len2 /\ addr2 < addr + len.
-
-Lemma overlaps_sym : forall addr1 len1 addr2 len2,
-  overlaps addr1 len1 addr2 len2 <-> overlaps addr2 len2 addr1 len1.
+Theorem Neq_out : n = m -> nat_of_N n = nat_of_N m.
 Proof.
-  split; intros;
-  destruct H; split; assumption.
+  intros H; apply (f_equal N.to_nat) in H;
+  autorewrite with N in *; assumption.
 Qed.
 
-Lemma not_overlaps_sym : forall addr1 len1 addr2 len2,
-  ~ overlaps addr1 len1 addr2 len2 <-> ~ overlaps addr2 len2 addr1 len1.
+Corollary Nneq_in : nat_of_N n <> nat_of_N m -> n <> m.
+Proof. congruence. Qed.
+
+Theorem Nneq_out : n <> m -> nat_of_N n <> nat_of_N m.
+Proof. intuition; apply Neq_in in H0; tauto. Qed.
+
+Theorem Nlt_in : (nat_of_N n < nat_of_N m)%nat -> n < m.
 Proof.
-  unfold not; split; intros;
-  apply overlaps_sym in H0;
-  contradiction.
+  unfold Nlt; intros.
+  rewrite nat_of_Ncompare.
+  apply (proj1 (nat_compare_lt _ _)); assumption.
 Qed.
 
-Lemma overlaps_irr : forall addr len1 len2,
-  0 < len1 -> 0 < len2 -> overlaps addr len1 addr len2.
+Theorem Nlt_out : n < m -> (nat_of_N n < nat_of_N m)%nat.
 Proof.
-  split; intros;
-  apply N.lt_add_pos_r; assumption.
+  unfold Nlt; intros.
+  rewrite nat_of_Ncompare in H.
+  apply nat_compare_Lt_lt; assumption.
 Qed.
 
-Ltac decisions :=
-  repeat
-    match goal with
-    | [ H : context [if ?B then _ else _] |- _ ] =>
-      let Heqe := fresh "Heqe" in
-      destruct B eqn:Heqe
-    | [ |- context [if ?B then _ else _] ] =>
-      let Heqe := fresh "Heqe" in
-      destruct B eqn:Heqe
-
-    | [ H : context[@IfDec_Then_Else _ _ _ _ _] |- _ ] =>
-      unfold IfDec_Then_Else in H; simpl in H
-    | [ |- context[@IfDec_Then_Else _ _ _ _ _] ] =>
-      unfold IfDec_Then_Else; simpl
-    end.
-
-Ltac undecide :=
-  repeat
-    match goal with
-    | [ H : is_true (_ <? _)  |- _ ] => apply N.ltb_lt in H
-    | [ H : (_ <? _) = true   |- _ ] => apply N.ltb_lt in H
-    | [ H : (_ <? _) = false  |- _ ] => apply N.ltb_ge in H
-    | [ H : is_true (_ <=? _) |- _ ] => apply N.leb_le in H
-    | [ H : (_ <=? _) = true  |- _ ] => apply N.leb_le in H
-    | [ H : (_ <=? _) = false |- _ ] => apply N.leb_gt in H
-    | [ H : is_true (_ =? _)  |- _ ] => apply N.eqb_eq in H; subst
-    | [ H : (_ =? _) = true   |- _ ] => apply N.eqb_eq in H; subst
-    | [ H : (_ =? _) = false  |- _ ] => apply N.eqb_neq in H
-
-    | [ |- is_true (_ <? _)  ] => apply N.ltb_lt
-    | [ |- (_ <? _) = true   ] => apply N.ltb_lt
-    | [ |- (_ <? _) = false  ] => apply N.ltb_ge
-    | [ |- is_true (_ <=? _) ] => apply N.leb_le
-    | [ |- (_ <=? _) = true  ] => apply N.leb_le
-    | [ |- (_ <=? _) = false ] => apply N.leb_gt
-    | [ |- is_true (_ =? _)  ] => apply N.eqb_eq
-    | [ |- (_ =? _) = true   ] => apply N.eqb_eq
-    | [ |- (_ =? _) = false  ] => apply N.eqb_neq
-    end.
-
-Ltac nomega_reduce :=
-  repeat (
-    match goal with
-    | [ H : (_ && _)%bool = true |- _ ] =>
-      apply Bool.andb_true_iff in H; destruct H
-    | [ H : (_ && _)%bool = false |- _ ] =>
-      apply Bool.andb_false_iff in H; destruct H
-
-    | [ H : { _ : N | _ } |- _ ] => destruct H; simpl in *
-
-    | [ H : _ <  _ <  _ |- _ ] => destruct H
-    | [ H : _ <= _ <  _ |- _ ] => destruct H
-    | [ H : _ <  _ <= _ |- _ ] => destruct H
-    | [ H : _ <= _ <= _ |- _ ] => destruct H
-
-    | [ |- _ <  _ <  _ ] => split
-    | [ |- _ <= _ <  _ ] => split
-    | [ |- _ <  _ <= _ ] => split
-    | [ |- _ <= _ <= _ ] => split
-
-    | [ H : ?N < ?M |- ?N < ?M + ?O ] => apply (N.lt_lt_add_r _ _ _ H)
-    | [ H : 0 < ?M  |- ?N < ?N + ?M ] => apply (N.lt_add_pos_r _ _ H)
-
-    | [ H : context[Z.of_N (_ + _)] |- _ ] => rewrite N2Z.inj_add in H
-    | [ H : context[Z.of_N (_ - _)] |- _ ] => rewrite N2Z.inj_sub in H; trivial
-
-    | [ |- context[Z.of_N (_ + _)] ] => rewrite N2Z.inj_add
-    | [ |- context[Z.of_N (_ - _)] ] => rewrite N2Z.inj_sub
-
-    | [ H : _ = _ |- _ ] => subst
-
-    | [ H : context[_ < _]  |- _ ] => rewrite N2Z.inj_lt in H
-    (* | [ H : context[_ = _]  |- _ ] => apply N2Z.inj_iff in H *)
-    (* | [ H : context[_ <> _] |- _ ] => apply N2Z.inj_iff in H *)
-
-    (* We need to give _ <= _ alone a chance to be used by N2Z.inj_sub. *)
-    | [ H : context[_     <= _ + _] |- _ ] => rewrite N2Z.inj_le in H
-    | [ H : context[_ + _ <= _    ] |- _ ] => rewrite N2Z.inj_le in H
-    | [ H : context[_ + _ <= _ + _] |- _ ] => rewrite N2Z.inj_le in H
-    | [ H : context[_     <= _    ] |- _ ] => rewrite N2Z.inj_le in H
-
-    | [ |- context[_ < _]  ] => rewrite N2Z.inj_lt
-    | [ |- context[_ <= _] ] => rewrite N2Z.inj_le
-    | [ |- context[_ = _]  ] => apply N2Z.inj_iff
-    | [ |- context[_ <> _] ] => apply N2Z.inj_iff
-    end; undecide).
-
-Ltac nomega := solve [ nomega_reduce; abstract omega ].
-
-Lemma overlaps_within : forall addr1 len1 addr2 len2,
-  0 < len1 -> overlaps addr1 len1 addr2 len2
-                <-> IfDec addr1 < addr2
-                    Then within addr1 len1 addr2
-                    Else within addr2 len2 addr1.
+Theorem Nle_in : (nat_of_N n <= nat_of_N m)%nat -> n <= m.
 Proof.
-  unfold overlaps, within.
-  split; intros.
-    destruct H0.
-    decisions; nomega.
-  decisions;
-  destruct H0.
-    nomega.
-  split; trivial.
-  undecide.
-  apply N.lt_eq_cases in Heqe.
-  destruct Heqe; nomega.
+  unfold Nle; intros.
+  rewrite nat_of_Ncompare.
+  apply (proj1 (nat_compare_le _ _)); assumption.
 Qed.
 
-Corollary not_overlaps_within : forall addr1 len1 addr2 len2,
-  0 < len1 -> ~ overlaps addr1 len1 addr2 len2
-                <-> IfDec addr1 < addr2
-                    Then ~ within addr1 len1 addr2
-                    Else ~ within addr2 len2 addr1.
+Theorem Nle_out : n <= m -> (nat_of_N n <= nat_of_N m)%nat.
 Proof.
-  split; intros.
-    decisions;
-    unfold not; intros;
-    apply H0, overlaps_within; trivial;
-    decisions; firstorder.
-  unfold not; intros;
-  apply overlaps_within in H1; trivial;
-  decisions; firstorder.
+  unfold Nle; intros.
+  rewrite nat_of_Ncompare in H.
+  apply nat_compare_le; assumption.
 Qed.
 
-Theorem Nle_add_plus : forall n m o, 0 < o -> n <= m -> n <= m + o.
+Theorem Ngt_out : n > m -> (nat_of_N n > nat_of_N m)%nat.
+Proof.
+  unfold Ngt; intros.
+  rewrite nat_of_Ncompare in H.
+  apply nat_compare_gt; assumption.
+Qed.
+
+Theorem Ngt_in : (nat_of_N n > nat_of_N m)%nat -> n > m.
+Proof.
+  unfold Ngt; intros.
+  rewrite nat_of_Ncompare.
+  apply nat_compare_gt; assumption.
+Qed.
+
+Theorem Nge_out : n >= m -> (nat_of_N n >= nat_of_N m)%nat.
+Proof.
+  unfold Nge; intros.
+  rewrite nat_of_Ncompare in H.
+  apply nat_compare_ge; assumption.
+Qed.
+
+Theorem Nge_in : (nat_of_N n >= nat_of_N m)%nat -> n >= m.
+Proof.
+  unfold Nge; intros.
+  rewrite nat_of_Ncompare.
+  apply nat_compare_ge; assumption.
+Qed.
+
+Theorem Nle_add_plus : forall o, 0 < o -> n <= m -> n <= m + o.
 Proof.
   intros.
   rewrite <- (N.add_0_r n).
-  apply N.add_le_mono; nomega.
+  apply N.add_le_mono; congruence.
 Qed.
 
-Lemma Nsub_eq : forall x y n,
-  n <= x -> n <= y -> x - n = y - n -> x = y.
+Lemma Nsub_eq : forall o, o <= n -> o <= m -> n - o = m - o -> n = m.
 Proof.
   intros.
   apply N2Z.inj_iff in H1.
@@ -196,55 +115,292 @@ Proof.
   omega.
 Qed.
 
-Corollary Neq_impl_eq : forall a b : N, a = b <-> a = b.
+Corollary Neq_impl_eq : n = m <-> n = m.
 Proof. split; intros; assumption. Qed.
+
 Hint Resolve Neq_impl_eq.
 
-Corollary Nneq_impl_neq : forall a b : N, a <> b <-> a <> b.
+Corollary Nneq_impl_neq : n <> m <-> n <> m.
 Proof. split; intros; assumption. Qed.
+
 Hint Resolve Nneq_impl_neq.
+
+Lemma Nlt_dec : {n < m} + {~ n < m}.
+Proof.
+  destruct (N.compare n m) eqn:Heqe.
+  - right; congruence.
+  - left; congruence.
+  - right; congruence.
+Qed.
+
+Lemma Nle_dec : {n <= m} + {~ n <= m}.
+Proof.
+  destruct (N.compare n m) eqn:Heqe.
+  - left; congruence.
+  - left; congruence.
+  - right; congruence.
+Qed.
+
+Lemma Ngt_dec : {n > m} + {~ n > m}.
+Proof.
+  destruct (N.compare n m) eqn:Heqe.
+  - right; congruence.
+  - right; congruence.
+  - left; congruence.
+Qed.
+
+Lemma Nge_dec : {n >= m} + {~ n >= m}.
+Proof.
+  destruct (N.compare n m) eqn:Heqe.
+  - left; congruence.
+  - right; congruence.
+  - left; congruence.
+Qed.
+
+End N_theory.
 
 Theorem Nle_impossible : forall n m, 0 < m -> n + m <= n -> False.
 Proof.
   intros.
   rewrite <- (N.add_0_r n) in H0 at 2.
   apply N.add_le_mono_l in H0.
-  nomega.
+  apply Nlt_out in H.
+  apply Nle_out in H0.
+  omega.
 Qed.
 
 Theorem Nadd_minus : forall n m, n <= m -> n + (m - n) = m.
-Proof. intros; nomega. Qed.
+Proof.
+  intros.
+  apply Nle_out in H.
+  apply Neq_in.
+  autorewrite with N.
+  omega.
+Qed.
+
+(*** definitions ***)
+
+Definition within (addr : N) (len : N) (a : N) : Prop :=
+  addr <= a < addr + len.
+
+Definition fits (addr1 len1 addr2 len2 : N) : Prop :=
+  within addr1 len1 addr2 /\ within addr1 len1 (addr2 + len2).
+
+Definition overlaps (addr len addr2 len2 : N) : Prop :=
+  addr < addr2 + len2 /\ addr2 < addr + len.
+
+(*** tactics ***)
+
+Ltac nsimp :=
+  simpl; repeat progress (autorewrite with N; simpl).
+
+Ltac nsimp_H H :=
+  simpl in H; repeat progress (autorewrite with N in H; simpl in H).
+
+Hint Extern 3 (Decidable.decidable (_ = _)) => apply N.eq_decidable.
+Hint Extern 3 (Decidable.decidable (_ < _)) => apply N.lt_decidable.
+Hint Extern 3 (Decidable.decidable (_ <= _)) => apply N.le_decidable.
+
+Ltac norm_N_step :=
+  match goal with
+  | [ |- ~ _ ] => unfold not; intros
+
+  | [ H : is_true (_ <? _)  |- _ ] => apply N.ltb_lt in H
+  | [ H : (_ <? _) = true   |- _ ] => apply N.ltb_lt in H
+  | [ H : (_ <? _) = false  |- _ ] => apply N.ltb_ge in H
+  | [ H : is_true (_ <=? _) |- _ ] => apply N.leb_le in H
+  | [ H : (_ <=? _) = true  |- _ ] => apply N.leb_le in H
+  | [ H : (_ <=? _) = false |- _ ] => apply N.leb_gt in H
+  | [ H : is_true (_ =? _)  |- _ ] => apply N.eqb_eq in H; subst
+  | [ H : (_ =? _) = true   |- _ ] => apply N.eqb_eq in H; subst
+  | [ H : (_ =? _) = false  |- _ ] => apply N.eqb_neq in H
+
+  | [ |- is_true (_ <? _)  ] => apply N.ltb_lt
+  | [ |- (_ <? _) = true   ] => apply N.ltb_lt
+  | [ |- (_ <? _) = false  ] => apply N.ltb_ge
+  | [ |- is_true (_ <=? _) ] => apply N.leb_le
+  | [ |- (_ <=? _) = true  ] => apply N.leb_le
+  | [ |- (_ <=? _) = false ] => apply N.leb_gt
+  | [ |- is_true (_ =? _)  ] => apply N.eqb_eq
+  | [ |- (_ =? _) = true   ] => apply N.eqb_eq
+  | [ |- (_ =? _) = false  ] => apply N.eqb_neq
+
+  | [ H : _ /\ _ |- _ ] => destruct H
+
+  | [ H : is_true ((_ && _)%bool) |- _ ] =>
+    apply Bool.andb_true_iff in H; destruct H
+  | [ H : (_ && _)%bool = true |- _ ] =>
+    apply Bool.andb_true_iff in H; destruct H
+  | [ H : (_ && _)%bool = false |- _ ] =>
+    apply Bool.andb_false_iff in H; destruct H
+
+  | [ |- is_true ((_ && _)%bool)  ] => apply Bool.andb_true_iff; split
+  | [ |- (_ && _)%bool = true  ] => apply Bool.andb_true_iff; split
+  | [ |- (_ && _)%bool = false ] => apply Bool.andb_false_iff
+
+  | [ H : { _ : N | _ } |- _ ] => destruct H; simpl in *
+
+  | [ |- {?P /\ ?Q} + {~ (?P /\ ?Q)} ] => apply sumbool_split
+  | [ |- {?n =  ?m} + {?n <> ?m} ] => apply N.eq_dec
+  | [ |- {?n <  ?m} + {~ (?n <  ?m)} ] => apply Nlt_dec
+  | [ |- {?n <= ?m} + {~ (?n <= ?m)} ] => apply Nle_dec
+  | [ |- {?n >  ?m} + {~ (?n >  ?m)} ] => apply Ngt_dec
+  | [ |- {?n >= ?m} + {~ (?n >= ?m)} ] => apply Nge_dec
+
+  | [ H : ~ _ < _  |- _ ] => apply N.nlt_ge in H
+  | [ H : ~ _ <= _ |- _ ] => apply N.nle_gt in H
+
+  | [ H : _ <  _ <  _ |- _ ] => destruct H
+  | [ H : _ <= _ <  _ |- _ ] => destruct H
+  | [ H : _ <  _ <= _ |- _ ] => destruct H
+  | [ H : _ <= _ <= _ |- _ ] => destruct H
+
+  | [ H : ~ (?x <  ?y <  ?z) |- _ ] => apply Decidable.not_and in H
+  | [ H : ~ (?x <= ?y <  ?z) |- _ ] => apply Decidable.not_and in H
+  | [ H : ~ (?x <  ?y <= ?z) |- _ ] => apply Decidable.not_and in H
+  | [ H : ~ (?x <= ?y <= ?z) |- _ ] => apply Decidable.not_and in H
+
+  | [ |- ~ (?x <  ?y <  ?z) ] => apply Decidable.not_and
+  | [ |- ~ (?x <= ?y <  ?z) ] => apply Decidable.not_and
+  | [ |- ~ (?x <  ?y <= ?z) ] => apply Decidable.not_and
+  | [ |- ~ (?x <= ?y <= ?z) ] => apply Decidable.not_and
+
+  | [ H : ~ (?x <  ?y /\ ?w <  ?z) |- _ ] => apply Decidable.not_and in H
+  | [ H : ~ (?x <= ?y /\ ?w <  ?z) |- _ ] => apply Decidable.not_and in H
+  | [ H : ~ (?x <  ?y /\ ?w <= ?z) |- _ ] => apply Decidable.not_and in H
+  | [ H : ~ (?x <= ?y /\ ?w <= ?z) |- _ ] => apply Decidable.not_and in H
+
+  | [ |- ~ (?x <  ?y /\ ?w <  ?z) ] =>
+    apply LogicFacts.not_and_implication; intros
+  | [ |- ~ (?x <= ?y /\ ?w <  ?z) ] =>
+    apply LogicFacts.not_and_implication; intros
+  | [ |- ~ (?x <  ?y /\ ?w <= ?z) ] =>
+    apply LogicFacts.not_and_implication; intros
+  | [ |- ~ (?x <= ?y /\ ?w <= ?z) ] =>
+    apply LogicFacts.not_and_implication; intros
+
+  | [ |- _ <  _ <  _ ] => split
+  | [ |- _ <= _ <  _ ] => split
+  | [ |- _ <  _ <= _ ] => split
+  | [ |- _ <= _ <= _ ] => split
+
+  | [ H : ?n < ?m |- ?n < ?m + ?o ] => apply (N.lt_lt_add_r _ _ _ H)
+  | [ H : 0 < ?m  |- ?n < ?n + ?m ] => apply (N.lt_add_pos_r _ _ H)
+
+  | [ H : _ = _ |- _ ] => subst
+  end.
+
+Ltac norm_N := repeat progress (norm_N_step; auto).
+
+Ltac pre_nomega :=
+  unfold within, fits, overlaps in *;
+  nsimp; intros; norm_N; nsimp;
+  repeat
+    match goal with
+    | [ H : _ = _          |- _ ] => apply Neq_out in H; nsimp_H H
+    | [ H : _ <> _         |- _ ] => apply Nneq_out in H; nsimp_H H
+    | [ H : _ = _ -> False |- _ ] => apply Nneq_out in H; nsimp_H H
+    | [ H : _ < _          |- _ ] => apply Nlt_out in H; nsimp_H H
+    | [ H : _ <= _         |- _ ] => apply Nle_out in H; nsimp_H H
+    | [ H : _ > _          |- _ ] => apply Ngt_out in H; nsimp_H H
+    | [ H : _ >= _         |- _ ] => apply Nge_out in H; nsimp_H H
+
+    | [ |- _ = _  ] => apply Neq_in; nsimp
+    | [ |- _ < _  ] => apply Nlt_in; nsimp
+    | [ |- _ <= _ ] => apply Nle_in; nsimp
+    | [ |- _ > _  ] => apply Ngt_in; nsimp
+    | [ |- _ >= _ ] => apply Nge_in; nsimp
+    end.
+
+Ltac nomega' :=
+  pre_nomega;
+  repeat progress match goal with
+  | _ => omega || (unfold nat_of_P in *; simpl in *; omega)
+  | [ H : _ \/ _ |- _ ] => destruct H; nomega'
+  | [ |- _ /\ _ ] => split; intros; nomega'
+  | [ |- _ <-> _ ] => split; intros; nomega'
+  | [ |- _ \/ _ ] => first [ solve [ left; nomega' ]
+                           | solve [ right; nomega' ] ]
+  end.
+
+Ltac nomega := solve [ nomega' ].
+
+Ltac decisions :=
+  repeat
+    match goal with
+    | [ H : context [if ?B then _ else _] |- _ ] =>
+      let Heqe := fresh "Heqe" in destruct B eqn:Heqe
+    | [ |- context [if ?B then _ else _] ] =>
+      let Heqe := fresh "Heqe" in destruct B eqn:Heqe
+
+    | [ H : context[@IfDec_Then_Else _ _ _ _ _] |- _ ] =>
+      unfold IfDec_Then_Else in H; simpl in H
+    | [ |- context[@IfDec_Then_Else _ _ _ _ _] ] =>
+      unfold IfDec_Then_Else; simpl
+    end.
+
+(*** within ***)
+
+Lemma within_refl : forall addr len,
+  0 < len -> within addr len addr.
+Proof. nomega. Qed.
 
 Lemma within_reflect : forall x y a,
   within x y a <-> ((x <=? a) && (a <? x + y) = true)%bool.
-Proof.
-  intros.
-  unfold within.
-  split; intros; try nomega.
-  apply Bool.andb_true_iff; split; nomega.
-Qed.
+Proof. nomega. Qed.
 
 Lemma not_within_reflect : forall x y a,
   ~ within x y a <-> ((x <=? a) && (a <? x + y) = false)%bool.
-Proof.
-  intros.
-  unfold within.
-  split; intros; try nomega.
-  apply Bool.andb_false_iff.
-  apply Decidable.not_and in H.
-    destruct H.
-      left; nomega.
-    right; nomega.
-  unfold Decidable.decidable; nomega.
-Qed.
+Proof. nomega. Qed.
 
 Lemma within_dec : forall a l x,
   {within a l x} + {~ within a l x}.
+Proof. nomega. Qed.
+
+(*** fits ***)
+
+(*** overlaps ***)
+
+Lemma overlaps_sym : forall addr1 len1 addr2 len2,
+  overlaps addr1 len1 addr2 len2 <-> overlaps addr2 len2 addr1 len1.
+Proof. nomega. Qed.
+
+Lemma overlaps_trans : forall a b x y z,
+  y < z -> overlaps a b x y -> overlaps a b x z.
+Proof. nomega. Qed.
+
+Lemma not_overlaps_sym : forall addr1 len1 addr2 len2,
+  ~ overlaps addr1 len1 addr2 len2 <-> ~ overlaps addr2 len2 addr1 len1.
+Proof. nomega. Qed.
+
+Corollary not_overlaps_trans : forall a b x y z,
+  z < y -> ~ overlaps a b x y -> ~ overlaps a b x z.
+Proof. nomega. Qed.
+
+Lemma overlaps_irr : forall addr len1 len2,
+  0 < len1 -> 0 < len2 -> overlaps addr len1 addr len2.
+Proof. nomega. Qed.
+
+Lemma overlaps_within : forall addr1 len1 addr2 len2,
+  0 < len1 -> overlaps addr1 len1 addr2 len2
+                <-> IfDec addr1 < addr2
+                    Then within addr1 len1 addr2
+                    Else within addr2 len2 addr1.
+Proof. intros; decisions; nomega. Qed.
+
+Corollary not_overlaps_within : forall addr1 len1 addr2 len2,
+  0 < len1
+    -> ~ overlaps addr1 len1 addr2 len2
+         <-> IfDec addr1 < addr2
+             Then ~ within addr1 len1 addr2
+             Else ~ within addr2 len2 addr1.
 Proof.
-  intros.
-  destruct (Decidable.Decidable_witness (P:=within a l x)) eqn:Heqe.
-    apply within_reflect in Heqe.
-    left; assumption.
-  apply not_within_reflect in Heqe.
-  right; assumption.
+  split; intros.
+    decisions;
+    unfold not; intros;
+    apply H0, overlaps_within; trivial;
+    decisions; firstorder.
+  unfold not; intros;
+  apply overlaps_within in H1; trivial;
+  decisions; firstorder.
 Qed.
